theories/rules/rules_Mov.v
@@ -14,29 +14,29 @@ Section cap_lang_rules.
   Implicit Types r : RegName.
   Implicit Types v : cap_lang.val. 
   Implicit Types w : Word.
-  Implicit Types reg : gmap RegName Word.
+  Implicit Types reg : gmap (CoreN * RegName) Word.
   Implicit Types ms : gmap Addr Word.
 
-  Inductive Mov_spec (regs: Reg) (dst: RegName) (src: Z + RegName) (regs': Reg): cap_lang.val -> Prop :=
+  Inductive Mov_spec (i : CoreN) (regs: Reg) (dst: RegName) (src: Z + RegName) (regs': Reg): cap_lang.val -> Prop :=
   | IsPtr_spec_success w:
-      word_of_argument regs src = Some w →
-      incrementPC (<[ dst := w ]> regs) = Some regs' →
-      Mov_spec regs dst src regs' NextIV
+      word_of_argument regs i src = Some w →
+      incrementPC (<[ (i, dst) := w ]> regs) i = Some regs' →
+      Mov_spec i regs dst src regs' (i, NextIV)
   | Mov_spec_failure w:
-      word_of_argument regs src = Some w →
-      incrementPC (<[ dst := w ]> regs) = None →
-      Mov_spec regs dst src regs' FailedV.
+      word_of_argument regs i src = Some w →
+      incrementPC (<[ (i, dst) := w ]> regs) i = None →
+      Mov_spec i regs dst src regs' (i, FailedV).
 
-  Lemma wp_Mov Ep pc_p pc_b pc_e pc_a  w dst src regs :
+  Lemma wp_Mov Ep i pc_p pc_b pc_e pc_a  w dst src regs :
     decodeInstrW w = Mov dst src ->
     isCorrectPC (WCap pc_p pc_b pc_e pc_a) →
-    regs !! PC = Some (WCap pc_p pc_b pc_e pc_a) →
-    regs_of (Mov dst src) ⊆ dom _ regs →
+    regs !! (i, PC) = Some (WCap pc_p pc_b pc_e pc_a) →
+    regs_of_core (Mov dst src) i ⊆ dom _ regs →
     {{{ ▷ pc_a ↦ₐ w ∗
         ▷ [∗ map] k↦y ∈ regs, k ↦ᵣ y }}}
-      Instr Executable @ Ep
+      (i, Instr Executable) @ Ep
     {{{ regs' retv, RET retv;
-        ⌜ Mov_spec regs dst src regs' retv ⌝ ∗
+        ⌜ Mov_spec i regs dst src regs' retv ⌝ ∗
         pc_a ↦ₐ w ∗
         [∗ map] k↦y ∈ regs', k ↦ᵣ y }}}.
   Proof.
@@ -50,24 +50,25 @@ Section cap_lang_rules.
     iModIntro. iSplitR. by iPureIntro; apply normal_always_head_reducible.
     iNext. iIntros (e2 σ2 efs Hpstep).
     apply prim_step_exec_inv in Hpstep as (-> & -> & (c & -> & Hstep)).
-    iSplitR; auto. eapply step_exec_inv in Hstep; eauto.
+    iSplitR; auto. eapply core_step_exec_inv in Hstep; eauto.
     unfold exec in Hstep.
 
-    specialize (indom_regs_incl _ _ _ Dregs Hregs) as Hri. unfold regs_of in Hri.
-    destruct (Hri dst) as [wdst [H'dst Hdst]]. by set_solver+.
+    specialize (indom_regs_incl _ _ _ Dregs Hregs) as Hri. unfold regs_of_core in Hri.
+    destruct (Hri i dst) as [wdst [H'dst Hdst]]. by set_solver+.
 
-    assert (exists w, word_of_argument regs src = Some w) as [wsrc Hwsrc].
+    assert (exists w, word_of_argument regs i src = Some w) as [wsrc Hwsrc].
     { destruct src as [| r0]; eauto; cbn.
-      destruct (Hri r0) as [? [? ?]]. set_solver+. eauto. }
+      destruct (Hri i r0) as [? [? ?]]. set_solver+. eauto. }
 
     pose proof Hwsrc as Hwsrc'. eapply word_of_argument_Some_inv' in Hwsrc; eauto.
 
-    assert (exec_opt (Mov dst src) (r, m) = updatePC (update_reg (r, m) dst wsrc)) as HH.
+    assert (exec_opt (Mov dst src) i (r, m)
+            = updatePC i (update_reg (r, m) i dst wsrc)) as HH.
     { destruct Hwsrc as [ [? [? ?] ] | [? (? & ? & Hr') ] ]; simplify_eq; eauto.
       cbn. by rewrite /= Hr'. }
     rewrite HH in Hstep. rewrite /update_reg /= in Hstep.
 
-    destruct (incrementPC (<[ dst := wsrc ]> regs)) as [regs'|] eqn:Hregs';
+    destruct (incrementPC (<[ (i, dst) := wsrc ]> regs) i) as [regs'|] eqn:Hregs';
       pose proof Hregs' as H'regs'; cycle 1.
     { apply incrementPC_fail_updatePC with (m:=m) in Hregs'.
       eapply updatePC_fail_incl with (m':=m) in Hregs'.
@@ -76,187 +77,199 @@ Section cap_lang_rules.
       rewrite Hregs' in Hstep. simplify_pair_eq.
       iFrame. iApply "Hφ"; iFrame. iPureIntro. econstructor; eauto. }
 
-    eapply (incrementPC_success_updatePC _ m) in Hregs'
+    eapply (incrementPC_success_updatePC _ i m) in Hregs'
       as (p' & g' & b' & e' & a'' & a_pc' & HPC'' & HuPC & ->).
     eapply updatePC_success_incl with (m':=m) in HuPC. 2: by eapply insert_mono; eauto.
     rewrite HuPC in Hstep. simplify_pair_eq. iFrame.
-    iMod ((gen_heap_update_inSepM _ _ dst) with "Hr Hmap") as "[Hr Hmap]"; eauto.
-    iMod ((gen_heap_update_inSepM _ _ PC) with "Hr Hmap") as "[Hr Hmap]"; eauto.
+    iMod ((gen_heap_update_inSepM _ _ (i, dst)) with "Hr Hmap") as "[Hr Hmap]"; eauto.
+    iMod ((gen_heap_update_inSepM _ _ (i, PC)) with "Hr Hmap") as "[Hr Hmap]"; eauto.
     iFrame. iModIntro. iApply "Hφ". iFrame. iPureIntro. econstructor; eauto.
   Qed.
 
-  Lemma wp_move_success_z E pc_p pc_b pc_e pc_a pc_a' w r1 wr1 z :
+  Lemma wp_move_success_z E i pc_p pc_b pc_e pc_a pc_a' w r1 wr1 z :
     decodeInstrW w = Mov r1 (inl z) →
     isCorrectPC (WCap pc_p pc_b pc_e pc_a) →
     (pc_a + 1)%a = Some pc_a' →
 
-    {{{ ▷ PC ↦ᵣ WCap pc_p pc_b pc_e pc_a
+    {{{ ▷ (i, PC) ↦ᵣ WCap pc_p pc_b pc_e pc_a
         ∗ ▷ pc_a ↦ₐ w
-        ∗ ▷ r1 ↦ᵣ wr1 }}}
-      Instr Executable @ E
-      {{{ RET NextIV;
-          PC ↦ᵣ WCap pc_p pc_b pc_e pc_a'
+        ∗ ▷ (i, r1) ↦ᵣ wr1 }}}
+      (i, Instr Executable) @ E
+      {{{ RET (i, NextIV);
+          (i, PC) ↦ᵣ WCap pc_p pc_b pc_e pc_a'
           ∗ pc_a ↦ₐ w
-          ∗ r1 ↦ᵣ WInt z }}}.
+          ∗ (i, r1) ↦ᵣ WInt z }}}.
   Proof.
     iIntros (Hinstr Hvpc Hpca' ϕ) "(>HPC & >Hpc_a & >Hr1) Hφ".
     iDestruct (map_of_regs_2 with "HPC Hr1") as "[Hmap %]".
-    iApply (wp_Mov with "[$Hmap Hpc_a]"); eauto; simplify_map_eq; eauto.
+    iApply (wp_Mov with "[$Hmap Hpc_a]"); eauto; simplify_map_eq by simplify_pair_eq; eauto.
     by unfold regs_of; rewrite !dom_insert; set_solver+.
     iNext. iIntros (regs' retv) "(#Hspec & Hpc_a & Hmap)". iDestruct "Hspec" as %Hspec.
 
     destruct Hspec as [|].
     { (* Success *)
-      iApply "Hφ". iFrame. incrementPC_inv; simplify_map_eq.
-      rewrite (insert_commute _ PC r1) // insert_insert insert_commute // insert_insert.
+      iApply "Hφ". iFrame. incrementPC_inv ; simplify_map_eq by simplify_pair_eq.
+      rewrite (insert_commute _ (i, PC) (i, r1)) ; simplify_pair_eq.
+      rewrite insert_insert insert_commute ; simplify_pair_eq.
+      rewrite insert_insert ; simplify_pair_eq.
       iDestruct (regs_of_map_2 with "Hmap") as "(?&?)"; eauto; iFrame. }
     { (* Failure (contradiction) *)
-      incrementPC_inv; simplify_map_eq; eauto. congruence. }
+      incrementPC_inv; simplify_map_eq by simplify_pair_eq; eauto.
+      congruence. }
   Qed.
 
-  Lemma wp_move_success_reg E pc_p pc_b pc_e pc_a pc_a' w r1 wr1 rv wrv :
+  Lemma wp_move_success_reg E i pc_p pc_b pc_e pc_a pc_a' w r1 wr1 rv wrv :
     decodeInstrW w = Mov r1 (inr rv) →
     isCorrectPC (WCap pc_p pc_b pc_e pc_a) →
     (pc_a + 1)%a = Some pc_a' →
 
-    {{{ ▷ PC ↦ᵣ WCap pc_p pc_b pc_e pc_a
+    {{{ ▷ (i, PC) ↦ᵣ WCap pc_p pc_b pc_e pc_a
         ∗ ▷ pc_a ↦ₐ w
-        ∗ ▷ r1 ↦ᵣ wr1
-        ∗ ▷ rv ↦ᵣ wrv }}}
-      Instr Executable @ E
-      {{{ RET NextIV;
-          PC ↦ᵣ WCap pc_p pc_b pc_e pc_a'
+        ∗ ▷ (i, r1) ↦ᵣ wr1
+        ∗ ▷ (i, rv) ↦ᵣ wrv }}}
+      (i, Instr Executable) @ E
+      {{{ RET (i, NextIV);
+          (i, PC) ↦ᵣ WCap pc_p pc_b pc_e pc_a'
           ∗ pc_a ↦ₐ w
-          ∗ r1 ↦ᵣ wrv
-          ∗ rv ↦ᵣ wrv }}}.
+          ∗ (i, r1) ↦ᵣ wrv
+          ∗ (i, rv) ↦ᵣ wrv }}}.
   Proof.
     iIntros (Hinstr Hvpc Hpca' ϕ) "(>HPC & >Hpc_a & >Hr1 & >Hrv) Hφ".
     iDestruct (map_of_regs_3 with "HPC Hr1 Hrv") as "[Hmap (%&%&%)]".
-    iApply (wp_Mov with "[$Hmap Hpc_a]"); eauto; simplify_map_eq; eauto.
-    by unfold regs_of; rewrite !dom_insert; set_solver+.
+    iApply (wp_Mov with "[$Hmap Hpc_a]"); eauto; simplify_map_eq by simplify_pair_eq; eauto.
+    by unfold regs_of_core; rewrite !dom_insert; set_solver+.
     iNext. iIntros (regs' retv) "(#Hspec & Hpc_a & Hmap)". iDestruct "Hspec" as %Hspec.
 
     destruct Hspec as [|].
     { (* Success *)
-      iApply "Hφ". iFrame. incrementPC_inv; simplify_map_eq.
-      rewrite (insert_commute _ PC r1) // insert_insert (insert_commute _ PC r1) // insert_insert.
+      iApply "Hφ". iFrame. incrementPC_inv; simplify_map_eq by simplify_pair_eq.
+      rewrite (insert_commute _ (i, PC) (i, r1)) ; simplify_pair_eq.
+      rewrite insert_insert insert_commute ; simplify_pair_eq.
+      rewrite insert_insert ; simplify_pair_eq.
       iDestruct (regs_of_map_3 with "Hmap") as "(?&?&?)"; eauto; iFrame. }
-    { (* Failure (contradiction) *)
-      incrementPC_inv; simplify_map_eq; eauto. congruence. }
+   { (* Failure (contradiction) *)
+      incrementPC_inv; simplify_map_eq by simplify_pair_eq; eauto.
+      congruence. }
   Qed.
 
-  Lemma wp_move_success_reg_same E pc_p pc_b pc_e pc_a pc_a' w r1 wr1 :
+  Lemma wp_move_success_reg_same E i pc_p pc_b pc_e pc_a pc_a' w r1 wr1 :
     decodeInstrW w = Mov r1 (inr r1) →
     isCorrectPC (WCap pc_p pc_b pc_e pc_a) →
     (pc_a + 1)%a = Some pc_a' →
 
-    {{{ ▷ PC ↦ᵣ WCap pc_p pc_b pc_e pc_a
+    {{{ ▷ (i, PC) ↦ᵣ WCap pc_p pc_b pc_e pc_a
         ∗ ▷ pc_a ↦ₐ w
-        ∗ ▷ r1 ↦ᵣ wr1 }}}
-      Instr Executable @ E
-      {{{ RET NextIV;
-          PC ↦ᵣ WCap pc_p pc_b pc_e pc_a'
+        ∗ ▷ (i, r1) ↦ᵣ wr1 }}}
+      (i, Instr Executable) @ E
+      {{{ RET (i, NextIV);
+          (i, PC) ↦ᵣ WCap pc_p pc_b pc_e pc_a'
           ∗ pc_a ↦ₐ w
-          ∗ r1 ↦ᵣ wr1 }}}.
+          ∗ (i, r1) ↦ᵣ wr1 }}}.
   Proof.
     iIntros (Hinstr Hvpc Hpca' ϕ) "(>HPC & >Hpc_a & >Hr1) Hφ".
     iDestruct (map_of_regs_2 with "HPC Hr1") as "[Hmap %]".
-    iApply (wp_Mov with "[$Hmap Hpc_a]"); eauto; simplify_map_eq; eauto.
-    by unfold regs_of; rewrite !dom_insert; set_solver+.
+    iApply (wp_Mov with "[$Hmap Hpc_a]"); eauto; simplify_map_eq by simplify_pair_eq; eauto.
+    by unfold regs_of_core; rewrite !dom_insert; set_solver+.
     iNext. iIntros (regs' retv) "(#Hspec & Hpc_a & Hmap)". iDestruct "Hspec" as %Hspec.
 
     destruct Hspec as [|].
     { (* Success *)
-      iApply "Hφ". iFrame. incrementPC_inv; simplify_map_eq.
-      rewrite (insert_commute _ PC r1) // insert_insert insert_commute // insert_insert.
+      iApply "Hφ". iFrame. incrementPC_inv; simplify_map_eq by simplify_pair_eq.
+      rewrite (insert_commute _ (i, PC) (i, r1)) ; simplify_pair_eq.
+      rewrite insert_insert insert_commute ; simplify_pair_eq.
+      rewrite insert_insert ; simplify_pair_eq.
       iDestruct (regs_of_map_2 with "Hmap") as "(?&?)"; eauto; iFrame. }
     { (* Failure (contradiction) *)
-      incrementPC_inv; simplify_map_eq; eauto. congruence. }
+      incrementPC_inv; simplify_map_eq by simplify_pair_eq; eauto.
+      congruence. }
   Qed.
 
-  Lemma wp_move_success_reg_samePC E pc_p pc_b pc_e pc_a pc_a' w :
+  Lemma wp_move_success_reg_samePC E i pc_p pc_b pc_e pc_a pc_a' w :
     decodeInstrW w = Mov PC (inr PC) →
     isCorrectPC (WCap pc_p pc_b pc_e pc_a) →
     (pc_a + 1)%a = Some pc_a' →
 
-    {{{ ▷ PC ↦ᵣ WCap pc_p pc_b pc_e pc_a
+    {{{ ▷ (i, PC) ↦ᵣ WCap pc_p pc_b pc_e pc_a
         ∗ ▷ pc_a ↦ₐ w }}}
-      Instr Executable @ E
-      {{{ RET NextIV;
-          PC ↦ᵣ WCap pc_p pc_b pc_e pc_a'
+      (i, Instr Executable) @ E
+      {{{ RET (i, NextIV);
+          (i, PC) ↦ᵣ WCap pc_p pc_b pc_e pc_a'
           ∗ pc_a ↦ₐ w }}}.
   Proof.
     iIntros (Hinstr Hvpc Hpca' ϕ) "(>HPC & >Hpc_a) Hφ".
     iDestruct (map_of_regs_1 with "HPC") as "Hmap".
-    iApply (wp_Mov with "[$Hmap Hpc_a]"); eauto; simplify_map_eq; eauto.
-    by unfold regs_of; rewrite !dom_insert; set_solver+.
+    iApply (wp_Mov with "[$Hmap Hpc_a]"); eauto; simplify_map_eq by simplify_pair_eq; eauto.
+    by unfold regs_of_core; rewrite !dom_insert; set_solver+.
     iNext. iIntros (regs' retv) "(#Hspec & Hpc_a & Hmap)". iDestruct "Hspec" as %Hspec.
 
     destruct Hspec as [|].
     { (* Success *)
-      iApply "Hφ". iFrame. incrementPC_inv; simplify_map_eq.
+      iApply "Hφ". iFrame. incrementPC_inv; simplify_map_eq by simplify_pair_eq.
       rewrite !insert_insert.
       iDestruct (regs_of_map_1 with "Hmap") as "?"; eauto; iFrame. }
     { (* Failure (contradiction) *)
-      incrementPC_inv; simplify_map_eq; eauto. congruence. }
+      incrementPC_inv; simplify_map_eq by simplify_pair_eq; eauto. congruence. }
   Qed.
 
-  Lemma wp_move_success_reg_toPC E pc_p pc_b pc_e pc_a w r1 p b e a a':
+  Lemma wp_move_success_reg_toPC E i pc_p pc_b pc_e pc_a w r1 p b e a a':
     decodeInstrW w = Mov PC (inr r1) →
     isCorrectPC (WCap pc_p pc_b pc_e pc_a) →
     (a + 1)%a = Some a' →
 
-    {{{ ▷ PC ↦ᵣ WCap pc_p pc_b pc_e pc_a
+    {{{ ▷ (i, PC) ↦ᵣ WCap pc_p pc_b pc_e pc_a
         ∗ ▷ pc_a ↦ₐ w
-        ∗ ▷ r1 ↦ᵣ WCap p b e a }}}
-      Instr Executable @ E
-      {{{ RET NextIV;
-          PC ↦ᵣ WCap p b e a'
+        ∗ ▷ (i, r1) ↦ᵣ WCap p b e a }}}
+      (i, Instr Executable) @ E
+      {{{ RET (i, NextIV);
+          (i, PC) ↦ᵣ WCap p b e a'
           ∗ pc_a ↦ₐ w
-          ∗ r1 ↦ᵣ WCap p b e a }}}.
+          ∗ (i, r1) ↦ᵣ WCap p b e a }}}.
   Proof.
     iIntros (Hinstr Hvpc Hpca' ϕ) "(>HPC & >Hpc_a & >Hr1) Hφ".
     iDestruct (map_of_regs_2 with "HPC Hr1") as "[Hmap %]".
-    iApply (wp_Mov with "[$Hmap Hpc_a]"); eauto; simplify_map_eq; eauto.
-    by unfold regs_of; rewrite !dom_insert; set_solver+.
+    iApply (wp_Mov with "[$Hmap Hpc_a]"); eauto; simplify_map_eq by simplify_pair_eq; eauto.
+    by unfold regs_of_core; rewrite !dom_insert; set_solver+.
     iNext. iIntros (regs' retv) "(#Hspec & Hpc_a & Hmap)". iDestruct "Hspec" as %Hspec.
 
     destruct Hspec as [|].
     { (* Success *)
-      iApply "Hφ". iFrame. incrementPC_inv; simplify_map_eq.
-      rewrite (insert_commute _ PC r1) // insert_insert insert_commute // insert_insert.
+      iApply "Hφ". iFrame. incrementPC_inv; simplify_map_eq by simplify_pair_eq.
+      rewrite insert_insert insert_insert.
       iDestruct (regs_of_map_2 with "Hmap") as "(?&?)"; eauto; iFrame. }
     { (* Failure (contradiction) *)
-      incrementPC_inv; simplify_map_eq; eauto. congruence. }
+      incrementPC_inv; simplify_map_eq by simplify_pair_eq; eauto.
+      congruence. }
   Qed.
 
-  Lemma wp_move_success_reg_fromPC E pc_p pc_b pc_e pc_a pc_a' w r1 wr1 :
+  Lemma wp_move_success_reg_fromPC E i pc_p pc_b pc_e pc_a pc_a' w r1 wr1 :
     decodeInstrW w = Mov r1 (inr PC) →
     isCorrectPC (WCap pc_p pc_b pc_e pc_a) →
     (pc_a + 1)%a = Some pc_a' →
 
-    {{{ ▷ PC ↦ᵣ WCap pc_p pc_b pc_e pc_a
+    {{{ ▷ (i, PC) ↦ᵣ WCap pc_p pc_b pc_e pc_a
         ∗ ▷ pc_a ↦ₐ w
-        ∗ ▷ r1 ↦ᵣ wr1 }}}
-      Instr Executable @ E
-      {{{ RET NextIV;
-          PC ↦ᵣ WCap pc_p pc_b pc_e pc_a'
+        ∗ ▷ (i, r1) ↦ᵣ wr1 }}}
+      (i, Instr Executable) @ E
+      {{{ RET (i, NextIV);
+          (i, PC) ↦ᵣ WCap pc_p pc_b pc_e pc_a'
           ∗ pc_a ↦ₐ w
-          ∗ r1 ↦ᵣ WCap pc_p pc_b pc_e pc_a }}}.
+          ∗ (i, r1) ↦ᵣ WCap pc_p pc_b pc_e pc_a }}}.
   Proof.
     iIntros (Hinstr Hvpc Hpca' ϕ) "(>HPC & >Hpc_a & >Hr1) Hφ".
     iDestruct (map_of_regs_2 with "HPC Hr1") as "[Hmap %]".
-    iApply (wp_Mov with "[$Hmap Hpc_a]"); eauto; simplify_map_eq; eauto.
-    by unfold regs_of; rewrite !dom_insert; set_solver+.
+    iApply (wp_Mov with "[$Hmap Hpc_a]"); eauto; simplify_map_eq by simplify_pair_eq; eauto.
+    by unfold regs_of_core; rewrite !dom_insert; set_solver+.
     iNext. iIntros (regs' retv) "(#Hspec & Hpc_a & Hmap)". iDestruct "Hspec" as %Hspec.
 
     destruct Hspec as [|].
     { (* Success *)
-      iApply "Hφ". iFrame. incrementPC_inv; simplify_map_eq.
-      rewrite (insert_commute _ PC r1) // insert_insert insert_commute // insert_insert.
+      iApply "Hφ". iFrame. incrementPC_inv; simplify_map_eq by simplify_pair_eq.
+      rewrite (insert_commute _ (i, r1) (i, PC)) ; simplify_pair_eq.
+      rewrite insert_insert insert_insert.
       iDestruct (regs_of_map_2 with "Hmap") as "(?&?)"; eauto; iFrame. }
     { (* Failure (contradiction) *)
-      incrementPC_inv; simplify_map_eq; eauto. congruence. }
+      incrementPC_inv; simplify_map_eq by simplify_pair_eq; eauto.
+      congruence. }
   Qed.
 
 End cap_lang_rules.
